Try Dafny's seq instead of own lists; proofs break

Compiler.dfy
@@ -20,24 +20,7 @@
 /* The instruction set of the machine. */
 
 datatype option<T> = Some(T) | None
-datatype list<T> = Nil | Cons(T, list<T>)
 type id = string
-
-// My append function (Leroy uses Coq lists)
-function append<T>(l1: list<T>, l2: list<T>): list<T>
-{
-  match l1
-  case Nil => l2
-  case Cons(x, xs) => Cons(x, append(xs, l2))
-}
-
-// My length function
-function length<T>(l: list<T>): nat
-{
-  match l
-  case Nil => 0
-  case Cons(_, xs) => 1 + length(xs)
-}
 
 datatype instruction =
   | Iconst(nat)
@@ -54,20 +37,19 @@ datatype instruction =
   | Ibgt(nat)
   | Ihalt
 
-type code = list<instruction>
+type code = seq<instruction>
 
 /* [code_at(C, pc) = Some i] if [i] is the instruction at position [pc]
   in the list of instructions [C]. */
 
 function code_at (C: code, pc: nat) : option<instruction>
 {
-  match (C, pc)
-  case (Nil, _)         => None
-  case (Cons(i, _), 0)  => Some(i)
-  case (Cons(_, C'), n) => code_at(C', n - 1)
+  if C == [] then None
+  else if pc == 0 then Some(C[0])
+  else code_at(C[1..], pc - 1)
 }
 
-type stack = list<nat>
+type stack = seq<nat>
 
 /* A state maps atoms to natural numbers*/
 type state = map<id, nat>
@@ -92,35 +74,35 @@ least predicate transition (C: code, conf1: configuration, conf2: configuration)
   match code_at(C, pc1)
   case Some(Iconst(n)) =>
       && pc2 == pc1 + 1
-      && stk2 == Cons(n, stk1)
+      && stk2 == [n] + stk1
       && st2 == st1
   case Some(Ivar(x)) =>
       && pc2 == pc1 + 1
       && x in st1 // TODO: this is different from Leroy
-      && stk2 == Cons(st1[x], stk1)
+      && stk2 == [st1[x]] + stk1
       && st2 == st1
   case Some(Isetvar(x)) =>
       exists v ::
       && pc2 == pc1 + 1
-      && stk1 == Cons(v, stk2)
+      && stk1 == [v] + stk2
       && st2 == st1[x:=v]
   case Some(Iadd) =>
       exists v1, v2, vs ::
       && pc2 == pc1 + 1
-      && stk1 == Cons(v2, Cons(v1, vs))
-      && stk2 == Cons(v1 + v2, vs)
+      && stk1 == [v2, v1] + vs
+      && stk2 == [v1 + v2] + vs
       && st1 == st2
   case Some(Isub) =>
       exists v1, v2, vs ::
       && pc2 == pc1 + 1
-      && stk1 == Cons(v2, Cons(v1, vs))
-      && stk2 == Cons(v1 - v2, vs)
+      && stk1 == [v2, v1] + vs
+      && stk2 == [v1 - v2] + vs
       && st1 == st2
   case Some(Imul) =>
       exists v1, v2, vs ::
       && pc2 == pc1 + 1
-      && stk1 == Cons(v2, Cons(v1, vs))
-      && stk2 == Cons(v1 * v2, vs)
+      && stk1 == [v2, v1] + vs
+      && stk2 == [v1 * v2] + vs
       && st1 == st2
   case Some(Ibranch_forward(ofs)) =>
       && pc2 == pc1 + 1 + ofs
@@ -133,22 +115,22 @@ least predicate transition (C: code, conf1: configuration, conf2: configuration)
       && st1 == st2
   case Some(Ibeq(ofs)) =>
       exists v1, v2 ::
-      && stk1 == Cons(v2, Cons(v1, stk2))
+      && stk1 == [v2, v1] + stk2
       && (if v1 == v2 then pc2 == pc1 + 1 - ofs else pc2 == pc1 + 1)
       && st1 == st2
   case Some(Ibne(ofs)) =>
       exists v1, v2 ::
-      && stk1 == Cons(v2, Cons(v1, stk2))
+      && stk1 == [v2, v1] + stk2
       && (if v1 == v2 then pc2 == pc1 + 1 else pc2 == pc1 + 1 + ofs)
       && st1 == st2
   case Some(Ible(ofs)) =>
       exists v1, v2 ::
-      && stk1 == Cons(v2, Cons(v1, stk2))
+      && stk1 == [v2, v1] + stk2
       && (if v1 < v2 then pc2 == pc1 + 1 + ofs else pc2 == pc1 + 1)
       && st1 == st2
   case Some(Ibgt(ofs)) =>
       exists v1, v2 ::
-      && stk1 == Cons(v2, Cons(v1, stk2))
+      && stk1 == [v2, v1] + stk2
       && (if v1 < v2 then pc2 == pc1 + 1 else pc2 == pc1 + 1 + ofs)
       && st1 == st2
   case Some(Ihalt) => false
@@ -176,7 +158,7 @@ predicate mach_terminates (C: code, s_init: state, s_fin: state)
 {
   exists pc ::
   && code_at(C, pc) == Some(Ihalt)
-  && star_transition(C, (0, Nil, s_init), (pc, Nil, s_fin))
+  && star_transition(C, (0, [], s_init), (pc, [], s_fin))
 }
 
 greatest predicate infseq_transition(C: code, conf: configuration)
@@ -186,7 +168,7 @@ greatest predicate infseq_transition(C: code, conf: configuration)
 
 predicate mach_diverges(C: code, s_init: state)
 {
-  infseq_transition(C, (0, Nil, s_init))
+  infseq_transition(C, (0, [], s_init))
 }
 
 predicate irred_transition(C: code, conf: configuration)
@@ -203,9 +185,9 @@ predicate irred_transition(C: code, conf: configuration)
 predicate mach_goes_wrong(C: code, s_init: state)
 {
   exists pc, stk, s_fin ::
-  && star_transition(C, (0, Nil, s_init), (pc, stk, s_fin))
+  && star_transition(C, (0, [], s_init), (pc, stk, s_fin))
   && irred_transition(C, (pc, stk, s_fin))
-  && (code_at(C, pc) != Some(Ihalt) || stk != Nil)
+  && (code_at(C, pc) != Some(Ihalt) || stk != [])
 }
 
 /* An important property of the virtual machine is that it is deterministic:
@@ -248,23 +230,23 @@ lemma terminates_unique(C: code, st: state, st1: state, st2: state)
   requires mach_terminates(C, st, st2)
   ensures st1 == st2
 {
-  var pc1 :| code_at(C, pc1) == Some(Ihalt) && star_transition(C, (0, Nil, st), (pc1, Nil, st1));
-  var pc2 :| code_at(C, pc2) == Some(Ihalt) && star_transition(C, (0, Nil, st), (pc2, Nil, st2));
-  finseq_unique(C, (0, Nil, st), (pc1, Nil, st1), (pc2, Nil, st2));
+  var pc1 :| code_at(C, pc1) == Some(Ihalt) && star_transition(C, (0, [], st), (pc1, [], st1));
+  var pc2 :| code_at(C, pc2) == Some(Ihalt) && star_transition(C, (0, [], st), (pc2, [], st2));
+  finseq_unique(C, (0, [], st), (pc1, [], st1), (pc2, [], st2));
 }
 
 lemma terminates_goeswrong_exclusive(C: code, st: state, st': state)
   requires mach_terminates(C, st, st')
   ensures !mach_goes_wrong(C, st)
 {
-  var pc :| code_at(C, pc) == Some(Ihalt) && star_transition(C, (0, Nil, st), (pc, Nil, st'));
-  var conf := (0, Nil, st);
-  var conf' := (pc, Nil, st');
+  var pc :| code_at(C, pc) == Some(Ihalt) && star_transition(C, (0, [], st), (pc, [], st'));
+  var conf := (0, [], st);
+  var conf' := (pc, [], st');
   forall stk_stuck, st_stuck, pc_stuck
-    | && star_transition(C, (0, Nil, st), (pc_stuck, stk_stuck, st_stuck))
+    | && star_transition(C, (0, [], st), (pc_stuck, stk_stuck, st_stuck))
       && irred_transition(C, (pc_stuck, stk_stuck, st_stuck))
     ensures && pc == pc_stuck
-            && stk_stuck == Nil
+            && stk_stuck == []
             {
               finseq_unique(C, conf, conf', (pc_stuck, stk_stuck, st_stuck));
             }
@@ -305,9 +287,9 @@ lemma terminates_diverges_exclusive(C: code, st: state, st': state)
   requires mach_terminates(C, st, st')
   ensures !mach_diverges(C, st)
 {
-  var pc :| code_at(C, pc) == Some(Ihalt) && star_transition(C, (0, Nil, st), (pc, Nil, st'));
-  var conf := (0, Nil, st);
-  var conf' := (pc, Nil, st');
+  var pc :| code_at(C, pc) == Some(Ihalt) && star_transition(C, (0, [], st), (pc, [], st'));
+  var conf := (0, [], st);
+  var conf' := (pc, [], st');
   infseq_finseq_excl(C, conf, conf');
 }
 
@@ -315,11 +297,11 @@ lemma goeswrong_diverges_exclusive(C: code, st: state)
   requires mach_goes_wrong(C, st)
   ensures !mach_diverges(C, st)
 {
-  var conf := (0, Nil, st);
+  var conf := (0, [], st);
   var pc, stk, s_fin :|
     && star_transition(C, conf, (pc, stk, s_fin))
     && irred_transition(C, (pc, stk, s_fin))
-    && (code_at(C, pc) != Some(Ihalt) || stk != Nil);
+    && (code_at(C, pc) != Some(Ihalt) || stk != []);
   var conf' := (pc, stk, s_fin);
   infseq_finseq_excl(C, conf, conf');
 }
@@ -367,11 +349,11 @@ This is the familiar translation to "reverse Polish notation".
 function compile_aexp (a: aexp) : code
 {
   match a
-  case ANum(n) => Cons(Iconst(n), Nil)
-  case AId(v) => Cons(Ivar(v), Nil)
-  case APlus(a1, a2) => append(compile_aexp(a1), append(compile_aexp(a2), Cons(Iadd, Nil)))
-  case AMinus(a1, a2) => append(compile_aexp(a1), append(compile_aexp(a2), Cons(Isub, Nil)))
-  case AMult(a1, a2) => append(compile_aexp(a1), append(compile_aexp(a2), Cons(Imul, Nil)))
+  case ANum(n) => [Iconst(n)]
+  case AId(v) => [Ivar(v)]
+  case APlus(a1, a2) => compile_aexp(a1) + compile_aexp(a2) + [Iadd]
+  case AMinus(a1, a2) => compile_aexp(a1) + compile_aexp(a2) + [Isub]
+  case AMult(a1, a2) => compile_aexp(a1) + compile_aexp(a2) + [Imul]
 }
 
 /* Some examples. */
@@ -379,11 +361,11 @@ function compile_aexp (a: aexp) : code
 method example1()
 {
   var e1 := compile_aexp(APlus(AId(vx), ANum(1)));
-  var expected1 := Cons(Ivar(vx), Cons(Iconst(1), Cons(Iadd, Nil)));
+  var expected1 := [Ivar(vx), Iconst(1), Iadd];
   assert e1 == expected1;
 
   var e2 := compile_aexp(AMult(AId(vy), APlus(AId(vx), ANum(1))));
-  var expected2 := Cons(Ivar(vy), Cons(Ivar(vx), Cons(Iconst(1), Cons(Iadd, Cons(Imul, Nil)))));
+  var expected2 := [Ivar(vy), Ivar(vx), Iconst(1), Iadd, Imul];
   assert e2 == expected2;
 }
 
@@ -391,19 +373,19 @@ function compile_bexp(b: bexp, cond: bool, ofs: nat) : code
 {
   match b
   case BTrue =>
-      if cond then Cons(Ibranch_forward(ofs), Nil) else Nil
+      if cond then [Ibranch_forward(ofs)] else []
   case BFalse =>
-      if cond then Nil else Cons(Ibranch_forward(ofs), Nil)
+      if cond then [] else [Ibranch_forward(ofs)]
   case BEq(a1, a2) =>
-      append(compile_aexp(a1), append(compile_aexp(a2), if cond then Cons(Ibeq(ofs), Nil) else Cons(Ibne(ofs), Nil)))
+      compile_aexp(a1) + compile_aexp(a2) + if cond then [Ibeq(ofs)] else [Ibne(ofs)]
   case BLe(a1, a2) =>
-      append(compile_aexp(a1), append(compile_aexp(a2), if cond then Cons(Ible(ofs), Nil) else Cons(Ibgt(ofs), Nil)))
+      compile_aexp(a1) + compile_aexp(a2) + if cond then [Ible(ofs)] else [Ibgt(ofs)]
   case BNot(b1) =>
       compile_bexp(b1, !cond, ofs)
   case BAnd(b1, b2) =>
       var c2 := compile_bexp(b2, cond, ofs);
-      var c1 := compile_bexp(b1, false, if cond then length(c2) else ofs + length(c2));
-      append(c1, c2)
+      var c1 := compile_bexp(b1, false, if cond then |c2| else ofs + |c2|);
+      c1 + c2
 }
 
 /* Examples. */
@@ -411,15 +393,15 @@ function compile_bexp(b: bexp, cond: bool, ofs: nat) : code
 method example2()
 {
   var e1 := compile_bexp(BEq(AId(vx), ANum(1)), true, 42);
-  var expected1 := Cons(Ivar(vx), Cons(Iconst(1), Cons(Ibeq(42), Nil)));
+  var expected1 := [Ivar(vx), Iconst(1), Ibeq(42)];
   assert e1 == expected1;
 
   var e2 := compile_bexp(BAnd(BLe(ANum(1), AId(vx)), BLe(AId(vx), ANum(10))), false, 42);
-  var expected2 := Cons(Iconst(1), Cons(Ivar(vx), Cons(Ibgt(45), Cons(Ivar(vx), Cons(Iconst(10), Cons(Ibgt(42), Nil))))));
+  var expected2 := [Iconst(1), Ivar(vx), Ibgt(45), Ivar(vx), Iconst(10), Ibgt(42)];
   assert e2 == expected2;
 
   var e3 := compile_bexp(BNot(BAnd(BTrue, BFalse)), true, 42);
-  var expected3 := Cons(Ibranch_forward(42), Nil);
+  var expected3 := [Ibranch_forward(42)];
   assert e3 == expected3;
 }
 
@@ -435,25 +417,24 @@ function compile_com(c: com) : code
 {
   match c
   case CSkip =>
-      Nil
+      []
   case CAss(id, a) =>
-      append(compile_aexp(a), Cons(Isetvar(id), Nil))
+      compile_aexp(a) + [Isetvar(id)]
   case CSeq(c1, c2) =>
-      append(compile_com(c1), compile_com(c2))
+      compile_com(c1) + compile_com(c2)
   case CIf(b, ifso, ifnot) =>
       var code_ifso := compile_com(ifso);
       var code_ifnot := compile_com(ifnot);
-      append(compile_bexp(b, false, length(code_ifso) + 1),
-             append(code_ifso,
-                    Cons(Ibranch_forward(length(code_ifnot)),
-                         code_ifnot)))
+      compile_bexp(b, false, |code_ifso| + 1)
+      + code_ifso
+      + [Ibranch_forward(|code_ifnot|)]
+      + code_ifnot
   case CWhile(b, body) =>
       var code_body := compile_com(body);
-      var code_test := compile_bexp(b, false, length(code_body) + 1);
-      append(code_test,
-             append(code_body,
-                    Cons(Ibranch_backward(length(code_test) + length(code_body) + 1),
-                         Nil)))
+      var code_test := compile_bexp(b, false, |code_body| + 1);
+      code_test
+      + code_body
+      + [Ibranch_backward(|code_test| + |code_body| + 1)]
 }
 
 /* The code for a program [p] (a command) is similar, but terminates
@@ -461,7 +442,7 @@ function compile_com(c: com) : code
 
 function compile_program(p: com): code
 {
-  append(compile_com(p), Cons(Ihalt, Nil))
+  compile_com(p) + [Ihalt]
 }
 
 /* Examples of compilation. */
@@ -469,15 +450,104 @@ function compile_program(p: com): code
 method example3()
 {
   var e1 := compile_program(CAss(vx, APlus(AId(vx), ANum(1))));
-  var expected1 := Cons(Ivar(vx), Cons(Iconst(1), Cons(Iadd, Cons(Isetvar(vx), Cons(Ihalt, Nil)))));
+  var expected1 := [Ivar(vx), Iconst(1), Iadd, Isetvar(vx), Ihalt];
   assert e1 == expected1;
 
   var e2 := compile_program(CWhile(BTrue, CSkip));
-  var expected2 := Cons(Ibranch_backward(1), Cons(Ihalt, Nil));
+  var expected2 := [Ibranch_backward(1), Ihalt];
   assert e2 == expected2;
 
   var e3 := compile_program(CIf(BEq(AId(vx), ANum(1)), CAss(vx, ANum(0)), CSkip));
-  var expected3 := Cons(Ivar(vx), Cons(Iconst(1), Cons(Ibne(3), Cons(Iconst(0), Cons(Isetvar(vx), Cons(Ibranch_forward(0), Cons(Ihalt, Nil)))))));
+  var expected3 := [Ivar(vx), Iconst(1), Ibne(3), Iconst(0), Isetvar(vx), Ibranch_forward(0), Ihalt];
   assert e3 == expected3; 
 }
 
+/* 3. Semantic preservation */
+
+/* Auxiliary results about code sequences. */
+
+/* To reason about the execution of compiled code, we need to consider
+  code sequences [C2] that are at position [pc] in a bigger code
+  sequence [C = C1 ++ C2 ++ C3].  The following predicate
+  [codeseq_at C pc C2] does just this. */
+
+least predicate codeseq_at(C: code, pc: nat, C2: code)
+{
+  exists C1, C3 :: pc == |C1| && C == C1 + C2 + C3
+}
+
+/* We show a number of no-brainer lemmas about [code_at] and [codeseq_at],
+  then populate a "hint database" so that Coq can use them automatically. */
+
+// I'm concerned about the effect this will have on the Dafny proof:
+// the fact that we can't have a hint database.
+
+lemma code_at_app(i: instruction, c2: code, c1: code, pc: nat)
+  requires pc == |c1|
+  ensures code_at(c1 + [i] + c2, pc) == Some(i)
+{}
+
+lemma codeseq_at_head(C: code, pc: nat, i: instruction, C': code)
+requires codeseq_at(C, pc, [i] + C')
+ensures code_at(C, pc) == Some(i)
+{
+  forall C1, C3
+  | pc == |C1| && C == C1 + [i] + C' + C3
+  {
+    code_at_app(i, C' + C3, C1, pc);
+  }
+}
+
+// Another difference with Coq: no type inference; function signatures have to be written in full
+// One more difference: arguments to lemmas have to be passed explicitly
+
+lemma codeseq_at_tail(C: code, pc: nat, i: instruction, C': code)
+requires codeseq_at(C, pc, [i] + C')
+ensures codeseq_at(C, pc + 1, C')
+{
+  forall C1, C3
+      | pc == |C1| && C == C1 + [i] + C' + C3
+      ensures codeseq_at(C, pc + 1, C')
+  {
+    var C1' := C1 + [i];
+    assert pc + 1 == |C1'|;
+    assert C == C1' + C' + C3;
+  }
+}
+
+// Lemma codeseq_at_tail:
+//   forall C pc i C',
+//   codeseq_at C pc (i :: C') ->
+//   codeseq_at C (pc + 1) C'.
+// Proof.
+//   intros. inversion H. 
+//   change (C1 ++ (i :: C') ++ C3)
+//     with (C1 ++ (i :: []) ++ C' ++ C3).
+//   rewrite <- app_ass. constructor. rewrite app_length. auto.
+// Qed. 
+
+// Lemma codeseq_at_app_left:
+//   forall C pc C1 C2,
+//   codeseq_at C pc (C1 ++ C2) ->
+//   codeseq_at C pc C1.
+// Proof.
+//   intros. inversion H. rewrite app_ass. constructor. auto.
+// Qed.
+
+// Lemma codeseq_at_app_right:
+//   forall C pc C1 C2,
+//   codeseq_at C pc (C1 ++ C2) ->
+//   codeseq_at C (pc + length C1) C2.
+// Proof.
+//   intros. inversion H. rewrite app_ass. rewrite <- app_ass. constructor. rewrite app_length. auto.
+// Qed.
+
+// Lemma codeseq_at_app_right2:
+//   forall C pc C1 C2 C3,
+//   codeseq_at C pc (C1 ++ C2 ++ C3) ->
+//   codeseq_at C (pc + length C1) C2.
+// Proof.
+//   intros. inversion H. repeat rewrite app_ass. rewrite <- app_ass. constructor. rewrite app_length. auto.
+// Qed.
+
+// Hint Resolve codeseq_at_head codeseq_at_tail codeseq_at_app_left codeseq_at_app_right codeseq_at_app_right2: codeseq.
